Quave/qreg.lean
@@ -1,0 +1,4 @@
+/-
+This file outlines the structure of a quantum register
+and definitions related to this structure.
+-/
