Quave/quantum.lean
@@ -1,0 +1,14 @@
+/-
+
+This file defines fundamental mathematical objects needed for quantum
+information and computation.
+
+  (a) Common States
+  (b) Common Gates
+    (i) Pauli Gates (I,X,Y,Z)
+    (ii) Hadamard Gate
+    (iii) Controlled-Not (CNOT)
+    (iv) Phase Gates
+    (v) Rotation Gates
+
+-/
